partial proof of pagedb preservation accross evalMOVSPCLRUC

verified/entry.i.dfy
@@ -1,187 +1,5 @@
 include "entry.s.dfy"
-
-/*
-predicate weakEquiv(d:PageDb,d':PageDb)
-    requires validPageDb(d) && validPageDb(d')
-{
-    (forall p | validPageNr(p) :: 
-        d[p].PageDbEntryTyped? <==> d'[p].PageDbEntryTyped?) &&
-    (forall p | validPageNr(p) && d[p].PageDbEntryTyped? ::
-        d[p].addrspace == d'[p].addrspace) &&
-    (forall p | validPageNr(p) && d[p].PageDbEntryTyped? ::
-        d[p].entry.Addrspace?  <==> d'[p].entry.Addrspace? &&
-        d[p].entry.Dispatcher? <==> d'[p].entry.Dispatcher? &&
-        d[p].entry.L1PTable?   <==> d'[p].entry.L1PTable? &&
-        d[p].entry.L2PTable?   <==> d'[p].entry.L2PTable?)
-}
-
-lemma equivUpToEnteredImpliesWeakEquiv(d:PageDb,d':PageDb,p':PageNr)
-    requires nonStoppedL1(d,p') && nonStoppedL1(d',p') &&
-        equivalentExceptPage(d,d',p')
-    ensures weakEquiv(d,d')
-{
-    forall ( p | validPageNr(p)) 
-        ensures d[p].PageDbEntryTyped? <==> d'[p].PageDbEntryTyped?
-    {
-    }
-    forall (p | validPageNr(p) && d[p].PageDbEntryTyped?)
-        ensures d[p].addrspace == d'[p].addrspace
-    {
-        if(p == p'){
-        } else {
-            assert d[p] == d'[p];
-        }
-    }
-    forall (p | validPageNr(p) && d[p].PageDbEntryTyped?)
-        ensures 
-        (d[p].entry.Addrspace?  <==> d'[p].entry.Addrspace? &&
-        d[p].entry.Dispatcher? <==> d'[p].entry.Dispatcher? &&
-        d[p].entry.L1PTable?   <==> d'[p].entry.L1PTable? &&
-        d[p].entry.L2PTable?   <==> d'[p].entry.L2PTable?)
-    {
-        if(p == p'){
-            assert nonStoppedL1(d,p);
-            assert nonStoppedL1(d',p);
-        } else {
-            assert d[p] == d'[p];
-            assert d[p].entry == d'[p].entry;
-            assert (d[p].entry.Addrspace?  <==> d'[p].entry.Addrspace? &&
-                    d[p].entry.Dispatcher? <==> d'[p].entry.Dispatcher? &&
-                    d[p].entry.L1PTable?   <==> d'[p].entry.L1PTable? &&
-                    d[p].entry.L2PTable?   <==> d'[p].entry.L2PTable?);
-        }
-    }
-}
-
-lemma MIClosedOverEquivUpToEntered(hw:state,hw':state,d:PageDb,d':PageDb,p:PageNr)
-    requires ValidState(hw) && ValidState(hw') &&
-        nonStoppedL1(d, p) && nonStoppedL1(d', p)
-    requires equivalentExceptPage(d,d',p)
-    requires WSMemInvariantExceptAddrspaceAtPage(hw,hw',d ,p)
-    ensures  WSMemInvariantExceptAddrspaceAtPage(hw,hw',d',p)
-{
-    reveal_validPageDb();
-    equivUpToEnteredImpliesWeakEquiv(d,d',p);
-    forall(m | m in hw.m.addresses && address_is_secure(m))
-        ensures memSWrInAddrspace(d, p, m) <==> memSWrInAddrspace(d', p, m)
-    {
-        assert m in hw'.m.addresses;
-    }
-}
-
-lemma MIWeaklyTransitive(s1:SysState, s2:SysState, s3:SysState, d:PageDb, p:PageNr)
-    requires validSysState(s1) && validSysState(s2) && validSysState(s3) && nonStoppedL1(d, p)
-    requires WSMemInvariantExceptAddrspaceAtPage(s1.hw, s2.hw, d, p) &&
-        WSMemInvariantExceptAddrspaceAtPage(s2.hw, s3.hw, d, p)
-    ensures WSMemInvariantExceptAddrspaceAtPage(s1.hw, s3.hw, d, p)
-{
-}
-
-lemma MITransitive(s1:SysState, s2:SysState, s3:SysState, p:PageNr)
-    requires validSysState(s1) && validSysState(s2) && validSysState(s3) &&
-        nonStoppedL1(s1.d,p) && nonStoppedL1(s2.d,p) && nonStoppedL1(s3.d,p) 
-    requires equivalentExceptPage(s1.d,s2.d,p) && equivalentExceptPage(s2.d,s3.d,p) 
-    requires WSMemInvariantExceptAddrspaceAtPage(s1.hw, s2.hw, s1.d, p) &&
-        WSMemInvariantExceptAddrspaceAtPage(s2.hw, s3.hw, s2.d, p)
-    ensures WSMemInvariantExceptAddrspaceAtPage(s1.hw, s3.hw, s1.d, p)
-{
-    MIClosedOverEquivUpToEntered(s2.hw,s3.hw,s2.d,s1.d,p);
-    assert WSMemInvariantExceptAddrspaceAtPage(s2.hw, s3.hw, s1.d, p);
-    MIWeaklyTransitive(s1,s2,s3,s1.d,p);
-    assert WSMemInvariantExceptAddrspaceAtPage(s1.hw, s3.hw, s1.d, p);
-}
-
-*/
-
-/*
-lemma valEnterImpliesBRPres(s:SysState,s':SysState,dispPage:PageNr,
-    a1:int,a2:int,a3:int)
-    requires isUInt32(a1) && isUInt32(a2) && isUInt32(a3) && validSysState(s)
-    requires smc_enter(s.d, dispPage,a1,a2,a3).1 == KOM_ERR_SUCCESS()
-        && validEnter(s, s', dispPage,a1,a2,a3)
-    ensures validEnter(s,s',dispPage,a1,a2,a3) ==>
-        bankedRegsPreserved(s.hw, s'.hw)
-{
-    reveal_ValidRegState();
-    forall ( s2, s3, s4, s5 | validSysStates({s2,s3,s4,s5})
-        && preEntryEnter(s,s2,dispPage,a1,a2,a3)
-        && entryTransitionEnter(s2, s3)
-        && s4.d == s3.d && userspaceExecution(s3.hw, s4.hw, s3.d)
-        && validERTransition(s4, s5) &&
-            !s5.hw.conf.ex.none? && mode_of_state(s5.hw) != User
-        && validERTransition(s5, s')
-        && (s'.hw.regs[R0], s'.hw.regs[R1], s'.d) ==
-            exceptionHandled(s5)
-        && s'.hw.conf.scr.ns == NotSecure)
-        ensures bankedRegsPreserved(s.hw, s'.hw)
-    {
-        assert bankedRegsPreserved(s.hw,  s2.hw);
-        assert bankedRegsPreserved(s2.hw, s3.hw);
-        assert bankedRegsPreserved(s3.hw, s4.hw);
-        assert bankedRegsPreserved(s4.hw, s5.hw);
-        assert bankedRegsPreserved(s5.hw, s'.hw);
-    }
-}
-*/
-
-/*
-lemma validERImpliesMemInv(s:SysState, s':SysState)
-    requires validERTransition(s,s');
-    ensures nonStoppedL1(s.d, l1pOfDispatcher(s.d, s.g.g_cur_dispatcher));
-    ensures WSMemInvariantExceptAddrspaceAtPage(s.hw,s'.hw,s.d,
-        l1pOfDispatcher(s.d, s.g.g_cur_dispatcher));
-    // ensures equivalentExceptPage(s.d, s'.d, s.g.g_cur_dispatcher);
-{
-}
-*/
-
-/*
-lemma valEnterImpliesMInv(s:SysState,s':SysState,dispPage:PageNr,
-    a1:int,a2:int,a3:int)
-    requires isUInt32(a1) && isUInt32(a2) && isUInt32(a3) && validSysState(s)
-    requires smc_enter(s.d, dispPage,a1,a2,a3).1 == KOM_ERR_SUCCESS()
-    requires validEnter(s, s', dispPage,a1,a2,a3)
-    ensures
-        var p := l1pOfDispatcher(s.d, dispPage);
-        nonStoppedL1(s.d,p)
-        && validSysState(s')
-        && WSMemInvariantExceptAddrspaceAtPage(s.hw, s'.hw, s.d, p)
-{
-    var p := l1pOfDispatcher(s.d, dispPage);
-    assert nonStoppedL1(s.d, p);
-    reveal_ValidRegState();
-    forall ( s2, s3, s4 | validSysStates({s2,s3,s4})
-        && preEntryEnter(s,s2,dispPage,a1,a2,a3)
-        && entryTransitionEnter(s2, s3)
-        && s4.d == s3.d && userspaceExecution(s3.hw, s4.hw, s3.d)
-        && validERTransition(s4, s')
-        && (s'.hw.regs[R0], s'.hw.regs[R1], s'.d) ==
-            exceptionHandled(s4)
-        && s'.hw.conf.scr.ns == NotSecure)
-        ensures 
-            ValidState(s.hw) && ValidState(s'.hw) && nonStoppedL1(s.d, p) &&
-            WSMemInvariantExceptAddrspaceAtPage(s.hw, s'.hw, s.d, p)
-    {
-    /*
-        assert preEntryEnter(s,s2,dispPage,a1,a2,a3) ==> 
-            WSMemInvariantExceptAddrspaceAtPage(s.hw, s2.hw, s.d,p);
-        assert preEntryEnter(s,s2,dispPage,a1,a2,a3);
-        assert WSMemInvariantExceptAddrspaceAtPage(s.hw,  s2.hw, s.d, p);
-        
-        validERImpliesMemInv(s2,s3);
-        assert l1pOfDispatcher(s2.d, s2.g.g_cur_dispatcher) == p;
-        assert WSMemInvariantExceptAddrspaceAtPage(s2.hw, s3.hw, s2.d, p);
-        MITransitive(s, s2, s3, p);
-        assert WSMemInvariantExceptAddrspaceAtPage(s.hw, s3.hw, s.d, p);
-     
-        assert WSMemInvariantExceptAddrspaceAtPage(s3.hw, s4.hw, s.d, p);
-        assert WSMemInvariantExceptAddrspaceAtPage(s.hw, s4.hw, s.d, p);
-        
-        assert WSMemInvariantExceptAddrspaceAtPage(s.hw, s'.hw, s.d, p);
-        */
-    }
-}
-*/
+include "ptables.i.dfy"
 
 function exceptionHandled_premium(s:SysState) : (int, int, PageDb)
     requires validSysState(s)
@@ -223,36 +41,62 @@ lemma exceptionHandledValidPageDb(s:SysState)
 }
 
 /*
+lemma eqAddressesSameExtraction(m:memstate, m':memstate)
+    requires SaneMem(m) && SaneMem(m')
+    requires m.addresses == m'.addresses
+    ensures  secPagesPreserved(m, m')
+{
+}
+
+lemma secAddressesImplSecPagesPres(m:memstate,m':memstate)
+    requires SaneMem(m) && SaneMem(m')
+    requires secAddressesPreserved(m, m')
+    ensures  secPagesPreserved(m, m')
+{
+}
+
 lemma enterUserspacePreservesGlobals(s:state,r:state)
     requires ValidState(s) && evalEnterUserspace(s,r)
     ensures  s.m.globals == r.m.globals
+    ensures  s.m.addresses == r.m.addresses
 {
+    reveal_ValidMemState();
 }
 
 lemma userspaceExecutionPreservesGlobals(s:state,r:state)
     requires ValidState(s) && evalUserspaceExecution(s,r)
     ensures  s.m.globals == r.m.globals
+    ensures  s.m.addresses == r.m.addresses
 {
+    reveal_ValidMemState();
+    assume false;
 }
 
 lemma exceptionTakenPreservesGlobals(s:state, ex:exception, r:state)
     requires ValidState(s) && evalExceptionTaken(s, ex, r)
     ensures  s.m.globals == r.m.globals
+    ensures  s.m.addresses == r.m.addresses
 {
+    reveal_ValidMemState();
 }
 
 lemma appInvariantPreservesGlobals(s:state,r:state)
     requires ValidState(s) &&
         ApplicationUsermodeContinuationInvariant(s, r)
     ensures  s.m.globals == r.m.globals
+    ensures  s.m.addresses == r.m.addresses
 {
+    reveal_ValidMemState();
 }
 
 lemma evalMOVSPCLRUCPreservesGlobals(s:state, r:state)
-    requires AppStatePred(s) && evalMOVSPCLRUC(s, r)
+    requires ValidState(s)
+    requires SaneMem(s.m) && SaneMem(r.m) && evalMOVSPCLRUC(s, r)
     ensures  s.m.globals == r.m.globals
+    ensures secPagesPreserved(s.m, r.m)
 {
 
+    reveal_ValidMemState();
     forall ( ex, s2, s3, s4 | ValidState(s2) && ValidState(s3) && ValidState(s4)
         && evalEnterUserspace(s, s2)
         && evalUserspaceExecution(s2, s3)
@@ -260,17 +104,27 @@ lemma evalMOVSPCLRUCPreservesGlobals(s:state, r:state)
         && ApplicationUsermodeContinuationInvariant(s4, r)
         && r.ok )
     ensures s.m.globals == r.m.globals
+    ensures secPagesPreserved(s.m, r.m)
     {
         enterUserspacePreservesGlobals(s,s2);
         userspaceExecutionPreservesGlobals(s2,s3);
         exceptionTakenPreservesGlobals(s3,ex,s4);
         appInvariantPreservesGlobals(s4,r);
+        assert s.m.addresses == r.m.addresses;
+        eqAddressesSameExtraction(s.m, r.m);
     }
 }
 */
 
+predicate secPagesPreserved(m:memstate,m':memstate)
+{
+    SaneMem(m) && SaneMem(m') &&
+    forall p | validPageNr(p) :: extractPage(m, p) == extractPage(m', p)
+}
+
 lemma enterUserspacePreservesPageDb(d:PageDb,s:state,s':state)
-    requires SaneState(s) && SaneState(s') && validPageDb(d)
+    requires SaneMem(s.m) && SaneMem(s'.m) && validPageDb(d)
+        && ValidState(s) && ValidState(s')
     requires evalEnterUserspace(s, s')
     requires pageDbCorresponds(s.m, d)
     ensures  pageDbCorresponds(s'.m, d)
@@ -281,8 +135,85 @@ lemma enterUserspacePreservesPageDb(d:PageDb,s:state,s':state)
     reveal_pageContentsCorresponds();
 }
 
-lemma userspaceHavocPreservesPageDb(d:PageDb,s:state,s':state)
-    requires SaneState(s) && SaneState(s') && validPageDb(d)
+lemma nonWriteablePagesAreSafe(m:addr,s:state,s':state)
+    requires ValidState(s) && ValidState(s')
+    requires evalUserspaceExecution(s, s')
+    requires var pt := ExtractAbsPageTable(s);
+        pt.Just? && var pages := WritablePagesInTable(fromJust(pt));
+        BitwiseAnd(m, 0xffff_f000) !in pages
+    requires m in s.m.addresses
+    ensures s'.m.addresses[m] == s.m.addresses[m]
+{
+    reveal_ValidMemState();
+    reveal_ValidRegState();
+    var pt := ExtractAbsPageTable(s);
+    assert pt.Just?;
+    var pages := WritablePagesInTable(fromJust(pt));
+    assert s'.m.addresses[m] == havocPages(pages, s.m.addresses, s'.m.addresses)[m];
+    assert havocPages(pages, s.m.addresses, s'.m.addresses)[m] == s.m.addresses[m];
+}
+
+lemma onlyDataPagesAreWritable(p:PageNr,a:addr,d:PageDb,s:state, s':state)
+    requires PhysBase() == KOM_DIRECTMAP_VBASE()
+    requires ValidState(s) && ValidState(s') && evalUserspaceExecution(s,s')
+    requires validPageDb(d) && d[p].PageDbEntryTyped? && !d[p].entry.DataPage?
+    requires WordAligned(a)
+    requires addrInPage(a, p)
+    ensures var pt := ExtractAbsPageTable(s);
+        pt.Just? && var pages := WritablePagesInTable(fromJust(pt));
+        BitwiseAnd(a, 0xffff_f000) !in pages
+{
+    reveal_validPageDb();
+
+    var pt := ExtractAbsPageTable(s);
+    assert pt.Just?;
+    var pages := WritablePagesInTable(fromJust(pt));
+    var vbase := s.conf.ttbr0.ptbase + PhysBase();
+    assume address_is_secure(vbase);
+    assume PageAligned(vbase);
+    assert ExtractAbsL1PTable(s.m, vbase) == fromJust(pt);
+    var l1p := monvaddr_page(vbase);
+    assume BitwiseAnd(a,0xffff_f000) in pages <==> a in pages;
+    assume nonStoppedL1(d,l1p);
+    assume fromJust(pt) == mkAbsPTable(d, l1p);
+    assume WritablePagesInTable(fromJust(pt)) ==
+        WritablePagesInTable(mkAbsPTable(d, l1p));
+    
+    
+    forall( a':addr, p':PageNr | a' in WritablePagesInTable(fromJust(pt)) &&
+        addrInPage(a',p') )
+        ensures d[p'].PageDbEntryTyped? && d[p'].entry.DataPage?
+    {
+        lemma_writablePagesAreDataPages(p', a', d, l1p);
+    }
+    /*
+    assert a in pages ==>
+        d[p].PageDbEntryTyped? && d[p].entry.DataPage? by
+        {
+            assume a in pages <==> a in WritablePagesInTable(mkAbsPTable(d, l1p));
+            lemma_writablePagesAreDataPages(p, a, d, l1p);
+        }
+    */
+}
+
+lemma lemma_writablePagesAreDataPages(p:PageNr,a:addr,d:PageDb,l1p:PageNr)
+    requires PhysBase() == KOM_DIRECTMAP_VBASE()   
+    requires validPageDb(d)     
+    requires nonStoppedL1(d, l1p) 
+    requires PageAligned(a) && address_is_secure(a) 
+    requires a in WritablePagesInTable(mkAbsPTable(d, l1p)) 
+    requires addrInPage(a, p)
+    ensures  d[p].PageDbEntryTyped? && d[p].entry.DataPage?
+{
+    reveal_validPageDb();
+    reveal_pageDbEntryCorresponds();
+    reveal_pageContentsCorresponds();
+    lemma_WritablePages(d, l1p, a);
+}
+
+lemma userspaceExecutionPreservesPageDb(d:PageDb,s:state,s':state)
+    requires SaneMem(s.m) && SaneMem(s'.m) && validPageDb(d)
+        && ValidState(s) && ValidState(s')
     requires evalUserspaceExecution(s,s')
     requires pageDbCorresponds(s.m,  d)
     ensures  pageDbCorresponds(s'.m, d)
@@ -292,21 +223,60 @@ lemma userspaceHavocPreservesPageDb(d:PageDb,s:state,s':state)
     reveal_pageDbEntryCorresponds();
     reveal_pageContentsCorresponds();
 
+
     forall ( p | validPageNr(p) )
         ensures pageDbEntryCorresponds(d[p], extractPageDbEntry(s'.m,p));
-        ensures pageContentsCorresponds(p, d[p], extractPage(s'.m, p));
     {
         assert extractPageDbEntry(s.m, p) == extractPageDbEntry(s'.m, p);
         PageDbCorrespondsImpliesEntryCorresponds(s.m, d, p);
         assert pageDbEntryCorresponds(d[p], extractPageDbEntry(s.m, p));
         
+    }
+
+    var pt := ExtractAbsPageTable(s);
+    assert pt.Just?;
+
+    /*
+    assert pt == mkAbsPTable(d, s.conf.ttbr0.ptbase + PhysBase()) by
+    {
+        var vbase := s.conf.ttbr0.ptbase + PhysBase();
+        assert ValidAbsL1PTable(s.m, vbase);
+        lemma_ptablesMatch(s, d, vbase);
+    }
+    */
+
+
+    /*
+    forall( a | a in WritablePagesInTable(fromJust(pt)) )
+        ensures  forall p | addrInPage(a, p) ::
+            d[p].PageDbEntryTyped? && d[p].entry.DataPage?
+    {
+        assume false;
+    }
+    */
+
+    forall ( p | validPageNr(p) && d[p].PageDbEntryTyped? && 
+        !d[p].entry.DataPage? )
+        ensures pageContentsCorresponds(p, d[p], extractPage(s'.m, p));
+    {
+        forall ( a:addr | page_monvaddr(p) <= a < page_monvaddr(p) + PAGESIZE() )
+            ensures s'.m.addresses[a] == s.m.addresses[a]
+            {
+               var pt := ExtractAbsPageTable(s);
+               assert pt.Just?;
+               var pages := WritablePagesInTable(fromJust(pt));
+               onlyDataPagesAreWritable(p, a, d, s, s');
+               assert BitwiseAnd(a, 0xffff_f000) !in pages;
+               nonWriteablePagesAreSafe(a, s, s'); 
+            }
         assert extractPage(s.m, p) == extractPage(s'.m, p);
         assert pageContentsCorresponds(p, d[p], extractPage(s.m, p));
     }
 }
 
 lemma exceptionTakenPreservesPageDb(d:PageDb,s:state,ex:exception,s':state)
-    requires SaneState(s) && SaneState(s') && validPageDb(d)
+    requires SaneMem(s.m) && SaneMem(s'.m) && validPageDb(d)
+        && ValidState(s) && ValidState(s')
     requires evalExceptionTaken(s, ex, s')
     requires pageDbCorresponds(s.m, d)
     ensures  pageDbCorresponds(s'.m, d)
@@ -318,7 +288,8 @@ lemma exceptionTakenPreservesPageDb(d:PageDb,s:state,ex:exception,s':state)
 }
 
 lemma appInvariantPreservesPageDb(d:PageDb,s:state,s':state)
-    requires SaneState(s) && SaneState(s') && validPageDb(d)
+    requires SaneMem(s.m) && SaneMem(s'.m) && validPageDb(d)
+        && ValidState(s) && ValidState(s')
     requires ApplicationUsermodeContinuationInvariant(s, s')
     requires pageDbCorresponds(s.m , d)
     ensures  pageDbCorresponds(s'.m, d)
@@ -331,8 +302,8 @@ lemma appInvariantPreservesPageDb(d:PageDb,s:state,s':state)
 
 
 lemma evalMOVSPCLRUCPreservesPageDb(d:PageDb, s:state, r:state)
-    requires SaneState(s) && SaneState(r) && validPageDb(d)
-    requires thisIsKomodo()
+    requires ValidState(s) && ValidState(r)
+    requires SaneMem(s.m) && SaneMem(r.m) && validPageDb(d)
     requires evalMOVSPCLRUC(s, r) && pageDbCorresponds(s.m, d)
     ensures  pageDbCorresponds(r.m, d)
 
@@ -351,44 +322,9 @@ lemma evalMOVSPCLRUCPreservesPageDb(d:PageDb, s:state, r:state)
         ensures  pageDbCorresponds(r.m, d)
     {
         enterUserspacePreservesPageDb(d, s,  s2);
-        userspaceHavocPreservesPageDb(d, s2, s3); 
+        userspaceExecutionPreservesPageDb(d, s2, s3); 
         exceptionTakenPreservesPageDb(d, s3, ex, s4);
         appInvariantPreservesPageDb(d, s4, r);
     }
 }
 
-lemma MemInvarSubsumption(s:SysState,s':SysState,p:PageNr)
-    requires validSysState(s) && validSysState(s') && nonStoppedL1(s.d, p)
-    requires AllMemInvariant(s.hw,s'.hw) && s.d == s'.d
-    ensures  WSMemInvariantExceptAddrspaceAtPage(s.hw,s'.hw,s.d,p)
-{
-}
-
-/*
-predicate {:opaque} validEnter_premium(s:SysState,s':SysState,dispPage:PageNr,
-    a1:int,a2:int,a3:int)
-    requires isUInt32(a1) && isUInt32(a2) && isUInt32(a3) && validSysState(s)
-    requires smc_enter(s.d, dispPage, a1, a2, a3).1 == KOM_ERR_SUCCESS()
-    ensures validEnter_premium(s, s', dispPage,a1,a2,a3)
-        == validEnter(s, s', dispPage,a1,a2,a3)
-        /*
-    ensures (smc_enter(s.d, dispPage,a1,a2,a3).1 == KOM_ERR_SUCCESS()
-             && validEnter(s, s', dispPage,a1,a2,a3)) ==> 
-             */
-    ensures validEnter_premium(s, s', dispPage,a1,a2,a3) ==> 
-        var p := l1pOfDispatcher(s.d, dispPage);
-        nonStoppedL1(s.d, dispPage)
-        && validSysState(s')
-        && WSMemInvariantExceptAddrspaceAtPage(s.hw, s'.hw, s.d, p)
-        && bankedRegsPreserved(s.hw, s'.hw)
-{
-    if(validEnter(s, s',dispPage,a1,a2,a3)) then
-        valEnterImpliesMInv(s, s', dispPage,a1,a2,a3);
-        assert WSMemInvariantExceptAddrspaceAtPage(s.hw, s'.hw, s.d, 
-            l1pOfDispatcher(s.d,dispPage));
-        valEnterImpliesBRPres(s, s', dispPage,a1,a2,a3);
-        validEnter(s, s', dispPage,a1,a2,a3)
-    else
-        validEnter(s, s', dispPage,a1,a2,a3)
-}
-*/
